Normalization_Definitions.thy
@@ -1,0 +1,119 @@
+theory Normalization_Definitions
+  imports PDDL_Sema_Supplement
+begin
+
+text \<open> The only reason these are here instead of in their respective
+  normalization files is to reduce dependencies across files.
+  This benefits development on my low-RAM laptop.\<close>
+
+(* TODO think of a better name *)
+abbreviation "\<omega> \<equiv> Either [''object'']"
+
+(*
+- type hierarchy is empty (implicitly includes ''object'')
+- Everything else is Either [''object''].
+  This is a little superfluous: If well-formed, they can only be [''object'', ''object'', ...],
+    which is semantically equivalent to [''object'']
+  - predicate argument types are Either [''object''].
+  - const types are Either [''object'']
+  - actions parameters are detyped
+    This isn't superfluous because wf_action_schema does not ensure well-formed param types. *)
+definition (in ast_domain) typeless_dom :: "bool" where
+  "typeless_dom \<equiv>
+    types D = []
+    \<and> (\<forall>p \<in> set (predicates D). \<forall>T \<in> set (argTs p). T = \<omega>)
+    \<and> (\<forall>(n, T) \<in> set (consts D). T = \<omega>)
+    \<and> (\<forall>ac \<in> set (actions D). \<forall>(n, T) \<in> set (ac_params ac). T = \<omega>)"
+
+(*
+- domain is detyped
+- objects are detyped
+*)
+definition (in ast_problem) typeless_prob :: "bool" where
+  "typeless_prob \<equiv>
+    typeless_dom
+    \<and> (\<forall>(n, T) \<in> set (objects P). T = \<omega>)"
+
+definition (in ast_domain) "prec_normed_dom \<equiv>
+  \<forall>ac \<in> set (actions D). is_conj (ac_pre ac)"
+
+abbreviation (in ast_problem) "prec_normed_prob \<equiv> prec_normed_dom"
+
+definition (in ast_domain) "normalized_dom \<equiv>
+  typeless_dom \<and> prec_normed_dom"
+
+definition (in ast_problem) "normalized_prob \<equiv>
+  typeless_prob \<and> (is_conj (goal P)) \<and> prec_normed_prob"
+
+lemma (in ast_problem) normed_prob_normed_dom:
+  "normalized_prob \<Longrightarrow> normalized_dom"
+  unfolding normalized_prob_def normalized_dom_def typeless_prob_def by blast
+
+definition (in ast_domain) "relaxed_dom \<equiv>
+  normalized_dom \<and> (\<forall>a \<in> set (actions D). is_pos_conj (ac_pre a))"
+
+definition (in ast_problem) "relaxed_prob \<equiv>
+  normalized_prob \<and> is_pos_conj (goal P) \<and>
+    (\<forall>a \<in> set (actions D). is_pos_conj (ac_pre a))"
+
+(* contexts *)
+
+term wf_ast_problem
+
+locale normed_dom = wf_ast_domain D for D +
+  assumes normed_dom: normalized_dom
+
+locale normed_prob = wf_ast_problem P for P +
+  assumes normed_prob: normalized_prob
+
+sublocale normed_prob \<subseteq> normed_dom D
+  apply (unfold_locales)
+  using normed_prob normed_prob_normed_dom by simp
+
+(* reachability definitions *)
+
+definition (in ast_problem) applicable :: "plan_action \<Rightarrow> bool"
+  where "applicable \<pi> \<equiv> \<exists>\<pi>s M. plan_action_path I \<pi>s M \<and> \<pi> \<in> set \<pi>s"
+
+lemma (in ast_problem) applicable_alt:
+  "applicable \<pi> \<longleftrightarrow> (\<exists>\<pi>s M. plan_action_path I \<pi>s M \<and>
+    plan_action_enabled \<pi> M)"
+proof
+  assume "applicable \<pi>"
+  then obtain \<pi>s M where 1: "plan_action_path I \<pi>s M \<and> \<pi> \<in> set \<pi>s"
+    unfolding applicable_def by blast
+  then obtain \<pi>s' where "sublist_until \<pi>s \<pi> @ (\<pi> # \<pi>s') = \<pi>s"
+    using sublist_just_until by fastforce
+  with 1 show "\<exists>\<pi>s M. plan_action_path I \<pi>s M \<and>
+    plan_action_enabled \<pi> M"
+    using plan_action_path_append_elim plan_action_path_Cons by metis
+next
+  assume "\<exists>\<pi>s M. plan_action_path I \<pi>s M \<and> plan_action_enabled \<pi> M"
+  then obtain \<pi>s M where 1: "plan_action_path I \<pi>s M" "plan_action_enabled \<pi> M"
+    by auto
+  hence "plan_action_path M [\<pi>] (execute_plan_action \<pi> M)"
+    using plan_action_path_def plan_action_enabled_def
+    using execute_plan_action_def execute_ground_action_def by simp
+  moreover have "\<pi> \<in> set (\<pi>s @ [\<pi>])" by simp
+  ultimately show "applicable \<pi>" using 1 applicable_def plan_action_path_append_intro by fast
+qed
+
+definition (in ast_problem) achievable :: "object atom formula \<Rightarrow> bool"
+  where "achievable a \<equiv> \<exists>\<pi>s M. plan_action_path I \<pi>s M \<and> a \<in> M"
+
+lemma (in wf_ast_problem) achievable_predAtm:
+  "achievable a \<Longrightarrow> is_predAtom a"
+  unfolding achievable_def
+  using wf_I wf_plan_action_path wf_world_model_def
+  unfolding wf_fmla_atom_alt by meson
+
+
+
+
+
+
+
+
+
+
+end
